dataset/MBPP-DFY-50/dfy_files/task_id_239.dfy
@@ -1,0 +1,23 @@
+method NumberOfSequences(m: int, n: int) returns (count: int)
+    requires m > 0 && n > 0
+    ensures count >= 0
+{
+    var dp := new int[m+1, n+1];
+    for i := 0 to m+1
+    {
+        dp[i, 0] := 1;
+    }
+    for i := 1 to m+1
+    {
+        for j := 1 to n+1
+        {
+            var x := 0;
+            for k := 0 to i/2
+            {
+                x := x + dp[k, j-1];
+            }
+            dp[i, j] := x;
+        }
+    }
+    count := dp[m, n];
+}
