dataset/MBPP-DFY-50/dfy_files/task_id_281.dfy
@@ -1,0 +1,25 @@
+method AreElementsUnique(a: array<int>) returns (unique: bool)
+    requires a != null
+    ensures unique <==> forall i, j :: 0 <= i < j < a.Length ==> a[i] != a[j]
+    ensures !unique ==> exists i, j :: 0 <= i < j < a.Length && a[i] == a[j]
+{
+    unique := true;
+    for i := 0 to a.Length
+        invariant 0 <= i <= a.Length
+        invariant unique <==> forall k, l :: 0 <= k < l < i ==> a[k] != a[l]
+        invariant !unique ==> exists k, l :: 0 <= k < l < i && a[k] == a[l]
+    {
+        for j := i+1 to a.Length
+            invariant i < j <= a.Length
+            invariant unique <==> forall k :: 0 <= k < j ==> a[i] != a[k]
+            invariant !unique ==> exists k :: i < k < j && a[i] == a[k]
+        {
+            if a[i] == a[j]
+            {
+                unique := false;
+                break;
+            }
+        }
+        if(!unique) { break; }
+    }
+}
