dataset/MBPP-DFY-50/dfy_files/task_id_291.dfy
@@ -1,0 +1,28 @@
+method CountWays(n: int, k: int) returns (count: int)
+    requires n >= 0
+    requires k >= 0
+    ensures count >= 0
+{
+    if n == 0 then
+    {
+        count := 0;
+    }
+    else if n == 1 then
+    {
+        count := k;
+    }
+    else
+    {
+        var same := k;
+        var diff := k * (k - 1);
+        for i := 3 to n
+            invariant same >= 0
+            invariant diff >= 0
+        {
+            var temp := same;
+            same := diff;
+            diff := (same + diff) * (k - 1);
+        }
+        count := same + diff;
+    }
+}
