dataset/MBPP-DFY-50/dfy_files/task_id_295.dfy
@@ -1,0 +1,14 @@
+method SumOfDivisors(n: nat) returns (sum: nat)
+    requires n > 0
+    ensures sum >= n
+{
+    sum := 0;
+    for i := 1 to n + 1
+        invariant 1 <= i <= n + 1
+        invariant sum >= i - 1
+    {
+        if (n % i == 0) {
+            sum := sum + i;
+        }
+    }
+}
