dataset/MBPP-DFY-50/dfy_files/task_id_389.dfy
@@ -1,0 +1,23 @@
+method LucasNumber(n: int) returns (ln: int)
+    requires n >= 0
+    ensures ln == if n == 0 then 2 else if n == 1 then 1 else LucasNumber(n - 1) + LucasNumber(n - 2)
+{
+    if n == 0 {
+        ln := 2;
+    } else if n == 1 {
+        ln := 1;
+    } else {
+        var a := 2;
+        var b := 1;
+        for k := 2 to n
+            invariant 2 <= k <= n + 1
+            invariant a == LucasNumber(k - 2)
+            invariant b == LucasNumber(k - 1)
+        {
+            var tmp := a;
+            a := b;
+            b := tmp + b;
+        }
+        ln := b;
+    }
+}
