dataset/MBPP-DFY-50/dfy_files/task_id_394.dfy
@@ -1,0 +1,19 @@
+method ContainsNoDuplicates(seq: seq<int>) returns (result: bool)
+    ensures result <==> (forall i, j :: 0 <= i < j < |seq| ==> seq[i] != seq[j])
+{
+    result := true;
+    for i := 0 to |seq|
+        invariant 0 <= i <= |seq|
+        invariant result <==> (forall k, l :: 0 <= k < l < i ==> seq[k] != seq[l])
+    {
+        for j := i + 1 to |seq|
+            invariant i + 1 <= j <= |seq|
+            invariant result <==> (forall k :: i + 1 <= k < j ==> seq[i] != seq[k])
+        {
+            if seq[i] == seq[j] {
+                result := false;
+                return;
+            }
+        }
+    }
+}
