dataset/MBPP-DFY-50/dfy_files/task_id_395.dfy
@@ -1,0 +1,31 @@
+method FindFirstNonRepeatedChar(s: string) returns (found: bool, c: char)
+    ensures found ==> exists i :: 0 <= i < |s| && s[i] == c && (forall j :: 0 <= j < |s| && j != i ==> s[j] != c)
+    ensures !found ==> forall i, j :: 0 <= i < j < |s| ==> s[i] == s[j]
+{
+    found := false;
+    c := ' ';
+    var i := 0;
+    while i < |s| && !found
+        invariant 0 <= i <= |s|
+        invariant found ==> exists ii :: 0 <= ii < i && s[ii] == c && (forall jj :: 0 <= jj < i && jj != ii ==> s[jj] != c)
+        invariant !found ==> forall ii, jj :: 0 <= ii < jj < i ==> s[ii] == s[jj]
+    {
+        var j := 0;
+        var repeated := false;
+        while j < |s| && !repeated
+            invariant 0 <= j <= |s|
+            invariant repeated ==> s[i] == s[j] && i != j
+            invariant !repeated ==> forall jj :: 0 <= jj < j && jj != i ==> s[jj] != s[i]
+        {
+            if i != j && s[i] == s[j] {
+                repeated := true;
+            }
+            j := j + 1;
+        }
+        if !repeated {
+            found := true;
+            c := s[i];
+        }
+        i := i + 1;
+    }
+}
