dataset/MBPP-DFY-50/dfy_files/task_id_405.dfy
@@ -1,0 +1,14 @@
+method ContainsElement(seq: seq<int>, element: int) returns (result: bool)
+    ensures result <==> element in seq
+{
+    result := false;
+    for i := 0 to |seq|
+        invariant 0 <= i <= |seq|
+        invariant result <==> exists j :: 0 <= j < i && seq[j] == element
+    {
+        if seq[i] == element {
+            result := true;
+            break;
+        }
+    }
+}
