dataset/MBPP-DFY-50/dfy_files/task_id_415.dfy
@@ -1,0 +1,26 @@
+method FindMaxProductPair(a: array<int>) returns (index1: int, index2: int)
+    requires a != null
+    requires a.Length >= 2
+    ensures 0 <= index1 < index2 < a.Length
+    ensures forall i, j :: 0 <= i < j < a.Length ==> a[index1] * a[index2] >= a[i] * a[j]
+{
+    index1 := 0;
+    index2 := 1;
+    for i := 0 to a.Length
+        invariant 0 <= i <= a.Length
+        invariant 0 <= index1 < index2 < a.Length
+        invariant forall k, l :: 0 <= k < l < i ==> a[index1] * a[index2] >= a[k] * a[l]
+    {
+        for j := i + 1 to a.Length
+            invariant i < j <= a.Length
+            invariant 0 <= index1 < index2 < a.Length
+            invariant forall k, l :: 0 <= k < l < j ==> a[index1] * a[index2] >= a[k] * a[l]
+        {
+            if a[i] * a[j] > a[index1] * a[index2]
+            {
+                index1 := i;
+                index2 := j;
+            }
+        }
+    }
+}
