dataset/MBPP-DFY-50/dfy_files/task_id_428.dfy
@@ -1,0 +1,47 @@
+method ShellSort(a: array<int>)
+    requires a != null
+    modifies a
+    ensures a.Length == old(a.Length)
+    ensures IsSorted(a)
+    ensures multiset(a[..]) == multiset(old(a[..]))
+{
+    var n := a.Length;
+    var h := n / 2;
+    while h > 0
+        decreases h
+        invariant 0 <= h <= n
+        invariant h == 0 ==> IsSorted(a)
+        invariant multiset(a[..]) == multiset(old(a[..]))
+    {
+        for i := h to n - 1
+            decreases n - i
+            invariant h <= i < n
+            invariant IsHSort(a, h, i)
+            invariant multiset(a[..]) == multiset(old(a[..]))
+        {
+            var j := i;
+            while j >= h && a[j - h] > a[j]
+                decreases j
+                invariant h <= j < n
+                invariant a[j - h] > a[j] ==> IsHSort(a, h, j - 1)
+                invariant multiset(a[..]) == multiset(old(a[..]))
+            {
+                var temp := a[j];
+                a[j] := a[j - h];
+                a[j - h] := temp;
+                j := j - h;
+            }
+        }
+        h := h / 2;
+    }
+}
+
+predicate IsSorted(a: array<int>)
+{
+    forall i, j :: 0 <= i < j < a.Length ==> a[i] <= a[j]
+}
+
+predicate IsHSort(a: array<int>, h: int, until: int)
+{
+    forall i, j :: 0 <= i < j <= until && j % h == 0 ==> a[i] <= a[j]
+}
