dataset/MBPP-DFY-50/dfy_files/task_id_479.dfy
@@ -1,0 +1,28 @@
+method FirstDigit(n: int) returns (d: int)
+    requires n > 0
+    ensures 1 <= d <= 9
+    ensures d == n / Power10(NumberOfDigits(n) - 1)
+{
+    var m := n;
+    while m >= 10
+        invariant m >= d
+        invariant m >= 10
+    {
+        m := m / 10;
+    }
+    d := m;
+}
+
+function Power10(n: nat): (r: nat)
+    ensures r >= 1
+    ensures n > 0 ==> r % 10 == 0
+{
+	if (n == 0) then 1 else 10 * Power10(n-1)
+}
+
+function NumberOfDigits(n: nat) : (r: nat)
+    ensures r >= 1
+    ensures r == 1 <==> 0 <= n <= 9
+{
+    if 0 <= n <= 9 then 1 else 1+NumberOfDigits(n/10)
+}
