dataset/MBPP-DFY-50/dfy_files/task_id_589.dfy
@@ -1,0 +1,21 @@
+method PerfectSquaresBetween(start: int, end: int) returns (squares: seq<int>)
+    requires start >= 0 && end >= start
+    ensures forall i :: 0 <= i < |squares| ==> (exists j: int :: j * j == squares[i]) && start <= squares[i] <= end
+    ensures forall i :: start <= i <= end && (exists j: int :: j * j == i) ==> i in squares
+    {
+        squares := [];
+        var i := 0;
+        while (i * i < start)
+            invariant 0 <= i && i * i < start
+        {
+            i := i + 1;
+        }
+        while (i * i <= end)
+            invariant start <= i * i <= end + 1
+            invariant forall j :: 0 <= j < |squares| ==> (exists k: int :: k * k == squares[j]) && start <= squares[j] <= end
+            invariant forall j :: start <= j <= end && (exists k: int :: k * k == j) ==> j in squares
+        {
+            squares := squares + [i * i];
+            i := i + 1;
+        }
+    }
