dataset/MBPP-DFY-50/dfy_files/task_id_604.dfy
@@ -1,0 +1,28 @@
+function ReverseString(s: string): string
+    ensures |s| == |ReverseString(s)|
+    ensures forall i :: 0 <= i < |s| ==> s[i] == ReverseString(s)[|s| - 1 - i]
+{
+    var r := "";
+    for i := |s| - 1 downto 0
+    invariant 0 <= i < |s|
+    invariant |r| == |s| - i - 1
+    invariant forall j :: 0 <= j < |r| ==> r[j] == s[|s| - j - 1]
+    {
+        r := r + s[i];
+    }
+    return r;
+}
+
+method ReverseWords(s: string) returns (v: string)
+    ensures v == ReverseString(s)
+{
+    var words := s.Split(' ');
+    var reversedWords := "";
+    for i := |words| - 1 downto 0
+    invariant 0 <= i < |words|
+    invariant forall j :: 0 <= j < |reversedWords| ==> reversedWords[j] == words[|words| - j - 1]
+    {
+        reversedWords := reversedWords + " " + words[i];
+    }
+    return reversedWords;
+}
