dataset/MBPP-DFY-50/dfy_files/task_id_628.dfy
@@ -1,0 +1,23 @@
+method ReplaceSpacesWithPercent20(s: string) returns (v: string)
+    ensures |v| >= |s|
+    ensures forall i, j :: 0 <= i < |s| && 0 <= j < |v| && s[i] == ' ' ==> (v[j] == '%' && v[j+1] == '2' && v[j+2] == '0')
+    ensures forall i, j :: 0 <= i < |s| && 0 <= j < |v| && s[i] != ' ' ==> (v[j] == s[i])
+{
+    var s' : string := [];
+    for i := 0 to |s|
+    invariant 0 <= i <= |s|
+    invariant |s'| >= i
+    invariant forall k, l :: 0 <= k < i && 0 <= l < |s'| && s[k] == ' ' ==> (s'[l] == '%' && s'[l+1] == '2' && s'[l+2] == '0')
+    invariant forall k, l :: 0 <= k < i && 0 <= l < |s'| && s[k] != ' ' ==> (s'[l] == s[k])
+    {
+        if s[i] == ' '
+        {
+            s' := s' + ['%', '2', '0'];
+        }
+        else 
+        {
+            s' := s' + [s[i]];
+        }
+    }
+    return s';
+}
