dataset/MBPP-DFY-50/dfy_files/task_id_66.dfy
@@ -1,0 +1,21 @@
+predicate IsPositive(x: int)
+{
+    x > 0
+}
+
+method CountPositive(a: array<int>) returns (count: int)
+    requires a != null
+    ensures count >= 0
+    ensures count == | set i: int | 0 <= i < a.Length && IsPositive(a[i])|
+{
+    count := 0;
+    for i := 0 to a.Length
+        invariant 0 <= i <= a.Length
+        invariant count == | set j: int | 0 <= j < i && IsPositive(a[j])|
+    {
+        if IsPositive(a[i])
+        {
+            count := count + 1;
+        }
+    }
+}
