dataset/MBPP-DFY-50/dfy_files/task_id_93.dfy
@@ -1,0 +1,13 @@
+method Power(a: int, b: nat) returns (result: int)
+    ensures result == a ^^ b
+{
+    result := 1;
+    var i := 0;
+    while i < b
+        invariant 0 <= i <= b
+        invariant result == a ^^ i
+    {
+        result := result * a;
+        i := i + 1;
+    }
+}
