dataset/MBPP-DFY-50/src/task_id_472.dfy
@@ -1,7 +1,11 @@
 method ContainsConsecutiveNumbers(a: array<int>) returns (result: bool)
-  requires a.Length>0
   ensures result <==> (exists i :: 0 <= i < a.Length - 1 && a[i] + 1 == a[i + 1])
 {
+  if a.Length == 0
+  {
+    return false;
+  }
+
   result := false;
   for i := 0 to a.Length - 1
     invariant 0 <= i <= a.Length - 1
