dataset/MBPP-DFY-50/src/task_id_573.dfy
@@ -25,11 +25,7 @@ ghost function SetProduct(s : set<int>) : int
        x * SetProduct(s - {x})
 }
 
-/* 
- * This is necessary because, when we add one element, we need to make sure
- * that the product of the new set, as a whole, is the same as the product
- * of the old set times the new element.
- */
+
 lemma SetProductLemma(s: set <int>, x: int)
   requires x in s
   ensures SetProduct(s - {x}) * x == SetProduct(s)
